SV evaluator cleanup
  - Documentation for most evaluator.lisp functions

  - Added extralogical run-time errors for out-of-bounds indexing in
    4veclist-nth, renamed it to 4veclist-nth-safe

  - Added extralogical run-time errors to svex-apply for unknown functions or
    improper arity

  - Split svex-xeval out of evaluator.lisp into xeval.lisp

  - Split unused svex-eval-memotable stuff into junk.lisp

books/centaur/sv/svex/evaluator.lisp
@@ -38,7 +38,7 @@
 (local (in-theory (disable acl2::nth-when-zp)))
 
 (defxdoc evaluation
-  :parents (expression)
+  :parents (expressions)
   :short "Evaluation semantics of @(see svex) expressions.")
 
 (local (xdoc::set-default-parents evaluation))
@@ -48,28 +48,40 @@
   :true-listp t
   :parents (4vec))
 
-(define 4veclist-nth ((n natp) (x 4veclist-p))
+(define 4veclist-nth-safe ((n natp) (x 4veclist-p))
   :parents (4veclist)
-  :short "Like @(see nth) but with proper @(see fty-discipline) for @(see
-  4veclist)s."
+  :short "Like @(see nth) but, with proper @(see fty-discipline) for @(see
+4veclist)s.  ``Safely'' causes a run-time error if @('n') is out of bounds."
   :returns (elt 4vec-p)
   (mbe :logic (4vec-fix (nth n x))
-       :exec (or (nth n x) (4vec-x)))
+       :exec (or (nth n x)
+                 (raise "Index ~x0 too large for 4veclist of length ~x1." n (len x))
+                 (4vec-x)))
   ///
-  (deffixequiv 4veclist-nth
+  (deffixequiv 4veclist-nth-safe
     :hints(("Goal" :in-theory (enable 4veclist-fix))))
-  (defthm 4veclist-nth-of-nil
-    (equal (4veclist-nth n nil) (4vec-x))))
+
+  (defthm 4veclist-nth-safe-of-nil
+    (equal (4veclist-nth-safe n nil)
+           (4vec-x)))
+
+  (defthm 4veclist-nth-safe-of-cons
+    (implies (syntaxp (quotep n))
+             (equal (4veclist-nth-safe n (cons a b))
+                    (if (zp n)
+                        (4vec-fix a)
+                      (4veclist-nth-safe (1- n) b))))))
+
 
 (fty::defalist svex-env
   :key-type svar
   :val-type 4vec
   :true-listp t
-  :short "An alist mapping @(see svar)s to @(see 4vec)s.  Typically used as an
+  :short "An alist mapping @(see svar)s to @(see 4vec)s.  Often used as an
 environment that gives variables their values in @(see svex-eval)."
   ///
   (defthm svex-env-p-of-append
-    (implies (and (Svex-env-p x)
+    (implies (and (svex-env-p x)
                   (svex-env-p y))
              (svex-env-p (append x y)))
     :hints(("Goal" :in-theory (enable svex-env-p)))))
@@ -129,9 +141,10 @@ expect or preserve @(see fast-alists)."
   (mbe :logic (consp (hons-assoc-equal (svar-fix var) (svex-env-fix env)))
        :exec (consp (assoc-equal var env))))
 
-(define svex-env-fastlookup ((var svar-p) (env svex-env-p))
+(define svex-env-fastlookup ((var svar-p)
+                             (env svex-env-p "Must be a @(see fast-alist)."))
   :parents (svex-env)
-  :short "Fast lookup in an @(see svex-env), which must be a @(see fast-alist)."
+  :short "Fast lookup in a fast @(see svex-env)."
   :enabled t
   :guard-hints (("goal" :in-theory (enable svex-env-lookup)))
   (mbe :logic (svex-env-lookup var env)
@@ -183,122 +196,171 @@ expect or preserve @(see fast-alists)."
     (?         4vec-?              (test then else)    "if-then-else")
     (bit?      4vec-bit?           (test then else)    "bitwise if-then-else")))
 
-(defun svex-apply-collect-args (n max argsvar)
-  (declare (xargs :measure (nfix (- (nfix max) (nfix n)))))
-  (let* ((n (nfix n))
-         (max (nfix max)))
-    (if (zp (- max n))
-        nil
-      (cons `(4veclist-nth ,n ,argsvar)
-            (svex-apply-collect-args (+ 1 n) max argsvar)))))
+(encapsulate
+  ()
+  (local (defun syms->strings (x)
+           (if (atom (cdr x))
+               (list (symbol-name (car x)))
+             (cons (symbol-name (car x))
+                   (cons " "
+                         (syms->strings (cdr x)))))))
 
-(defun svex-apply-cases-fn (argsvar optable)
-  (b* (((when (atom optable)) '((otherwise (4vec-x))))
-       ((list sym fn args) (car optable))
-       (call `(,fn . ,(svex-apply-collect-args 0 (len args) argsvar))))
-    (cons `(,sym ,call)
-          (svex-apply-cases-fn argsvar (cdr optable)))))
+  (local (defun optable-to-xdoc-aux (optable acc)
+           ;; collects a reversed list of strings
+           (b* (((when (atom optable)) acc)
+                ((list name fn args descrip) (car optable))
+                (entry `("<tr><td>@('("
+                         ,@(syms->strings (cons name args))
+                         ")')</td><td>@(see " ,(symbol-name fn)
+                         ")</td><td>" ,descrip "</td></tr>" "
+")))
+             (optable-to-xdoc-aux (cdr optable) (revappend entry acc)))))
 
-(defmacro svex-apply-cases (fn args)
-  `(case ,fn
-     . ,(svex-apply-cases-fn args *svex-op-table*)))
+  (local (defun optable-to-xdoc ()
+           (declare (xargs :mode :program))
+           (str::fast-string-append-lst
+            `("<p>SVEX has a fixed language of known functions.
+The following table shows the function symbols (all in the
+SV package) and their meanings.</p>
+<table>
+<tr><th>SVEX form</th><th>4vec function</th><th>Description</th></tr>
+"
+              ,@(reverse (optable-to-xdoc-aux *svex-op-table* nil))
+              "</table>"))))
 
-(define svex-apply ((fn fnsym-p) (args 4veclist-p))
-  :short "Apply any known function to a list of @(see 4vec) arguments."
-  :long "<p>See @(see svex-functions) for the list of functions
-  recognized.</p>"
-  :returns (res 4vec-p)
+  (make-event
+   `(defxdoc svex-functions
+      :parents (expressions)
+      :short "The known svex functions symbols and their meanings."
+      :long ,(optable-to-xdoc))))
+
+
+(defsection svex-apply-cases
+  :parents (svex-apply)
+  :short "Generates the main case statement for @(see svex-apply)."
+  :long "@(def svex-apply-cases)"
+
+  (defun svex-apply-collect-args (n max argsvar)
+    (declare (xargs :measure (nfix (- (nfix max) (nfix n)))))
+    (let* ((n   (nfix n))
+           (max (nfix max)))
+      (if (zp (- max n))
+          nil
+        (cons `(4veclist-nth-safe ,n ,argsvar)
+              (svex-apply-collect-args (+ 1 n) max argsvar)))))
+
+  (defun svex-apply-cases-fn (argsvar optable)
+    (b* (((when (atom optable))
+          ;; Not a recognized function -- result is all Xes.
+          '((otherwise
+             (or (raise "Attempting to apply unknown function ~x0~%" fn)
+                 (4vec-x)))))
+         ((list sym fn args) (car optable))
+         (call `(mbe :logic
+                     (,fn . ,(svex-apply-collect-args 0 (len args) argsvar))
+                     :exec
+                     (let ((arity-check (or (eql (len args) ,(len args))
+                                            (raise "Improper arity for ~x0: expected ~x1 arguments but found ~x2.~%"
+                                                   ',sym ',(len args) (len args)))))
+                       (declare (ignore arity-check))
+                       (,fn . ,(svex-apply-collect-args 0 (len args) argsvar))))))
+      (cons `(,sym ,call)
+            (svex-apply-cases-fn argsvar (cdr optable)))))
+
+  (defmacro svex-apply-cases (fn args)
+    `(case ,fn
+       . ,(svex-apply-cases-fn args *svex-op-table*))))
+
+
+(define svex-apply
+  :short "Apply an @(see svex) function to some @(see 4vec) arguments."
+  ((fn   fnsym-p    "Name of the function to apply.")
+   (args 4veclist-p "Arguments to apply it to."))
+  :returns (result 4vec-p "Result of applying the function.")
+  :long "<p>This function captures function application for @(see svex-eval),
+using a big case statement on the @('fn') to execute.</p>
+
+<p>SVEX uses a fixed language of known functions with fixed arities; see @(see
+svex-functions) for the list of known functions and their meanings.  If we are
+given a known function of proper arity, we execute the corresponding 4vec
+operation on its arguments.</p>
+
+<ul>
+
+<li>Attempting to apply any unknown function produces an all-X result in the
+logic, and causes a run-time error during execution.</li>
+
+<li>Applying a function to the wrong number of arguments produces an all-X
+result in the logic, and causes a run-time error during execution.</li>
+
+</ul>"
+
   (let* ((fn (mbe :logic (fnsym-fix fn) :exec fn))
          (args (mbe :logic (4veclist-fix args) :exec args)))
     (svex-apply-cases fn args))
   ///
-  (deffixequiv svex-apply))
+  (deffixequiv svex-apply)
 
-(defun svcall-fn (fn args)
-  (declare (xargs :guard t))
-  (b* ((look (assoc fn *svex-op-table*))
-       ((unless look)
-        (er hard? 'svcall "Svex function doesn't exist: ~x0" fn))
-       (formals (third look))
-       ((unless (eql (len formals) (len args)))
-        (er hard? 'svcall "Wrong arity for call of ~x0" fn)))
-    `(svex-call ',fn (list . ,args))))
+  ;; Quick checks that arity checking and invalid function checking is working.
+  ;; BOZO it would be nice to do these with must-fail, but that doesn't seem
+  ;; to work.
 
-(defmacro svcall (fn &rest args)
-  (svcall-fn fn args))
+  ;; (svex-apply 'bad-function nil)
+  ;; (svex-apply 'id (list (4vec-x) (4vec-x)))
+  ;; (svex-apply 'id nil)
+  )
 
 
-
-;; (defthm svobj-p-when-4vec-p
-;;   (implies (4vec-p x)
-;;            (svobj-p x))
-;;   :hints(("Goal" :in-theory (enable svobj-p))))
-
-
-(local (defun syms->strings (x)
-         (if (atom (cdr x))
-             (list (symbol-name (car x)))
-           (cons (symbol-name (car x))
-                 (cons " "
-                       (syms->strings (cdr x)))))))
-
-(local (defun optable-to-xdoc-aux (optable acc)
-         ;; collects a reversed list of strings
-         (b* (((when (atom optable)) acc)
-              ((list name fn args descrip) (car optable))
-              (entry `("<tr><td>@('("
-                       ,@(syms->strings (cons name args))
-                       ")')</td><td>@(see " ,(symbol-name fn)
-                       ")</td><td>" ,descrip "</td></tr>" "
-")))
-           (optable-to-xdoc-aux (cdr optable) (revappend entry acc)))))
-
-(local (defun optable-to-xdoc ()
-         (declare (xargs :mode :program))
-         (str::fast-string-append-lst
-          `("<p>The following table shows the function symbols (all
-in the SVEX package) and their meanings.</p>
-<table>
-<tr><th>SVEX form</th><th>4vec function</th><th>Description</th></tr>
-"
-            ,@(reverse (optable-to-xdoc-aux *svex-op-table* nil))
-            "</table>"))))
-
-(make-event
- `(defxdoc svex-functions
-    :parents (svex)
-    :short "Svex function symbols and their meanings"
-    :long ,(optable-to-xdoc)))
 (defines svex-eval
-  :parents (svex)
-  :short "Concrete evaluation of svex formulas"
-  :long "<p>Svex-eval is a straightforward evaluator for svex formulas.  It
-takes an svex object and an environment mapping variables (@(see svar) objects)
-to @(see 4vec) values, and returns the 4vec value of the formula under that
-assignment in the obvious way.  Functions are applied using @(see svex-apply).
-Also see @(see svex-functions) for the list of recognized svex function symbols
-and their meanings.</p>"
+  :parents (evaluation)
+  :short "Evaluate an @(see svex) in some environment."
+
+  :long "<p>@('svex-eval') is a straightforward evaluator for @(see svex)
+formulas.  It takes as arguments an @(see svex) object to evaluate, and an
+environment mapping variables (@(see svar) objects) to @(see 4vec) values.  It
+returns the @(see 4vec) value of the formula, under this assignment, in the
+obvious way:</p>
+
+<ul>
+
+<li>Constants evaluate to themselves.</li>
+
+<li>Variables are looked up using @(see svex-env-fastlookup).  Note that any
+unbound variables evaluate to an infinite-width X.</li>
+
+<li>Functions applications are handled with @(see svex-apply).</li>
+
+</ul>
+
+<p>We typically expect @(see svex)es to be constructed with @(see hons).  To
+take advantage of this structure sharing, we @(see memoize) @(see
+svex-eval).</p>"
+
   :flag svex-eval-flag
   :flag-local nil
   :verify-guards nil
-  (define svex-eval ((x svex-p)
-                     (env svex-env-p))
-    ;; :guard (svex-aok x *svex-arity-table*)
+
+  (define svex-eval ((x   svex-p     "Expression to evaluate.")
+                     (env svex-env-p "Variable bindings.  Must be a @(see fast-alist)."))
     :measure (svex-count x)
     :flag expr
-    :returns (val 4vec-p :hints ((and stable-under-simplificationp
-                                       '(:expand ((4vec-p x))))))
+    :returns (val 4vec-p "Value of @('x') under this environment."
+                  :hints ((and stable-under-simplificationp
+                               '(:expand ((4vec-p x))))))
     (svex-case x
       :quote x.val
-      :var (svex-env-fastlookup x.name env)
-      :call (svex-apply x.fn (svexlist-eval x.args env))))
+      :var   (svex-env-fastlookup x.name env)
+      :call  (svex-apply x.fn (svexlist-eval x.args env))))
 
-  (define svexlist-eval ((x svexlist-p)
-                         (env svex-env-p))
-    ;; :guard (svex-aok-list x *svex-arity-table*)
+  (define svexlist-eval
+    :parents (evaluation)
+    :short "Evaluate each @(see svex) in a list under the same environment."
+    ((x   svexlist-p "List of expressions to evaluate.")
+     (env svex-env-p "Variable bindings.  Must be a @(see fast-alist)."))
+    :returns (vals 4veclist-p "Values of the expressions in @('x') under this environment.")
     :measure (svexlist-count x)
     :flag list
-    :returns (vals 4veclist-p)
+
     (if (atom x)
         nil
       (cons (svex-eval (car x) env)
@@ -306,103 +368,87 @@ and their meanings.</p>"
   ///
 
   (verify-guards svex-eval)
+  (memoize 'svex-eval :condition '(eq (svex-kind x) :call)))
 
-  (deffixequiv-mutual svex-eval
-    :hints (("goal" :expand ((svexlist-fix x)))))
+(defsection svexlist-eval-basics
+  :parents (svexlist-eval)
+  :short "Very basic list lemmas for @(see svexlist-eval)."
 
-  (defthm len-of-svexlist-eval
-    (equal (len (svexlist-eval x env))
-           (len x))
-    :hints(("Goal" :in-theory (enable svexlist-eval))))
+  (local (in-theory (enable svex-eval
+                            svexlist-eval)))
 
+  (defthm svexlist-eval-nil
+    (equal (svexlist-eval nil env)
+           nil))
 
   (defthm car-of-svexlist-eval
     (4vec-equiv (car (svexlist-eval x env))
-                 (svex-eval (car x) env))
-    :hints(("Goal" :in-theory (enable svexlist-eval))))
+                (svex-eval (car x) env)))
 
   (defthm cdr-of-svexlist-eval
     (4veclist-equiv (cdr (svexlist-eval x env))
-                     (svexlist-eval (cdr x) env))
-    :hints(("Goal" :in-theory (enable svexlist-eval))))
+                    (svexlist-eval (cdr x) env)))
 
-  (defthm svexlist-eval-nil
-    (equal (svexlist-eval nil env) nil))
+  (defthm svexlist-eval-of-cons
+    (equal (svexlist-eval (cons a b) env)
+           (cons (svex-eval a env)
+                 (svexlist-eval b env))))
+
+  (defthm len-of-svexlist-eval
+    (equal (len (svexlist-eval x env))
+           (len x)))
 
   (defthm svexlist-eval-of-append
     (equal (svexlist-eval (append a b) env)
            (append (svexlist-eval a env)
-                   (svexlist-eval b env)))
-    :hints(("Goal" :in-theory (enable append))))
+                   (svexlist-eval b env)))))
 
-  (memoize 'svex-eval :condition '(eq (svex-kind x) :call)))
-
-
-(defines svex-xeval
+(defsection svex-eval-basics
   :parents (svex-eval)
-  :short "Evaluate an svex under the empty (all-X) environment"
-  :long "<p>@('(svex-xeval x)') is the same as @('(svex-eval x nil)'), except
-that the case equality operator @('===') is treated as the (monotonic) equality
-operator @('==').  We provide a separate function for this special case because
-having a single argument improves memoization performance, and this function is
-commonly used in @(see svex-rewriting) to check whether a given expression only
-has one possible value.</p>"
-  :verify-guards nil
-  (define svex-xeval ((x svex-p))
-    :measure (svex-count x)
-    :returns (val 4vec-p)
-    (svex-case x
-      :quote x.val
-      :var (4vec-x)
-      :call (svex-apply
-             (if (eq x.fn '===)
-                 '==
-               x.fn)
-             (svexlist-xeval x.args))))
-  (define svexlist-xeval ((x svexlist-p))
-    :measure (svexlist-count x)
-    :returns (val 4veclist-p)
-    (if (atom x)
-        nil
-      (cons (svex-xeval (car x))
-            (svexlist-xeval (cdr x)))))
-  ///
-  (verify-guards svex-xeval)
+  :short "Very basic lemmas about @(see svex-eval)."
 
+  (local (in-theory (enable svex-eval
+                            svexlist-eval)))
 
-  (deffixequiv-mutual svex-xeval
+  "<h3>Congruence rules</h3>"
+
+  (deffixequiv-mutual svex-eval
     :hints (("goal" :expand ((svexlist-fix x)))))
 
-  (defthm len-of-svexlist-xeval
-    (equal (len (svexlist-xeval x))
-           (len x))
-    :hints(("Goal" :in-theory (enable svexlist-xeval))))
+  "<h3>Svex-eval of constants/constructors</h3>"
+
+  (make-event
+   `(encapsulate nil
+      (set-ignore-ok t)
+      (defthm svex-eval-of-quoted
+        (implies (syntaxp (quotep x))
+                 (equal (svex-eval x env)
+                        ,(acl2::body 'svex-eval nil (w state))))
+        :hints(("Goal" :in-theory (enable svex-eval))))))
+
+  (defthm svex-eval-of-svex-call
+    (equal (svex-eval (svex-call fn args) env)
+           (svex-apply fn (svexlist-eval args env)))
+    :hints(("Goal" :expand ((svex-eval (svex-call fn args) env)))))
+
+  (defthm svex-eval-when-fncall
+    (implies (equal (svex-kind x) :call)
+             (equal (svex-eval x env)
+                    (svex-apply (svex-call->fn x)
+                                (svexlist-eval (svex-call->args x) env))))
+    :hints(("Goal" :in-theory (enable svex-eval))))
+
+  (defthm svex-eval-when-quote
+    (implies (eq (svex-kind x) :quote)
+             (equal (svex-eval x env)
+                    (svex-quote->val x)))
+    :hints(("Goal" :in-theory (enable svex-eval)))))
 
 
-  (defthm car-of-svexlist-xeval
-    (4vec-equiv (car (svexlist-xeval x))
-                (svex-xeval (car x)))
-    :hints(("Goal" :in-theory (enable svexlist-xeval))))
 
-  (defthm cdr-of-svexlist-xeval
-    (4veclist-equiv (cdr (svexlist-xeval x))
-                    (svexlist-xeval (cdr x)))
-    :hints(("Goal" :in-theory (enable svexlist-xeval))))
-
-  (defthm svexlist-xeval-nil
-    (equal (svexlist-xeval nil) nil))
-
-  (defthm svexlist-xeval-of-append
-    (equal (svexlist-xeval (append a b))
-           (append (svexlist-xeval a)
-                   (svexlist-xeval b)))
-    :hints(("Goal" :in-theory (enable append))))
-
-  (memoize 'svex-xeval :condition '(eq (svex-kind x) :call)))
-
-
-
-(define svex-alist-eval-aux ((x svex-alist-p) (env svex-env-p))
+(define svex-alist-eval-aux ((x   svex-alist-p)
+                             (env svex-env-p))
+  :parents (svex-alist-eval)
   :prepwork ((local (in-theory (enable svex-alist-p svex-alist-fix svex-env-p))))
   :returns (xx svex-env-p :hints(("Goal" :in-theory (enable svex-env-p))))
   (if (atom x)
@@ -414,11 +460,18 @@ has one possible value.</p>"
               (svex-alist-eval-aux (cdr x) env))
       (svex-alist-eval-aux (cdr x) env))))
 
-
-
-(define svex-alist-eval ((x svex-alist-p) (env svex-env-p))
+(define svex-alist-eval
+  :parents (evaluation svex-alist)
+  :short "Evaluate every expression in an @(see svex-alist) under the same environment."
+  ((x   svex-alist-p "Alist of variables to @(see svex) expressions to evaluate.
+                      Need not be fast.")
+   (env svex-env-p   "Environment to evaluate the expressions under.  Should
+                      be a @(see fast-alist)."))
   :prepwork ((local (in-theory (enable svex-alist-p svex-alist-fix svex-env-p))))
-  :returns (xx svex-env-p :hints(("Goal" :in-theory (enable svex-env-p))))
+  :returns (result svex-env-p
+                   "New (slow) alist, binds the variables to their expressions'
+                    values."
+                   :hints(("Goal" :in-theory (enable svex-env-p))))
   :Verify-guards nil
   (mbe :logic
        (if (atom x)
@@ -453,99 +506,12 @@ has one possible value.</p>"
     :hints(("Goal" :in-theory (enable svex-alist-eval append)))))
 
 
-(defalist svex-memotable :key-type svex :val-type 4vec)
-
-(defthm 4vec-p-lookup-in-svex-memotable
-  (implies (and (svex-memotable-p x)
-                (hons-assoc-equal k x))
-           (4vec-p (cdr (hons-assoc-equal k x)))))
-
-(defines svex-eval-memo
-  ;; Self-memoized version of svex-eval, for GL
-  :verify-guards nil
-  (define svex-eval-memo ((x svex-p)
-                          (env svex-env-p)
-                          (memo svex-memotable-p))
-    :returns (mv (res 4vec-p)
-                 (memo1 svex-memotable-p))
-    :measure (svex-count x)
-    (b* ((memo (svex-memotable-fix memo)))
-      (svex-case x
-        :quote (mv x.val memo)
-        :var (mv (svex-env-fastlookup x.name env) memo)
-        :call (b* ((x (svex-fix x))
-                   (look (hons-get x memo))
-                   ((when look) (mv (cdr look) memo))
-                   ((mv args memo) (svexlist-eval-memo x.args env memo))
-                   (res (svex-apply x.fn args))
-                   (memo (hons-acons x res memo)))
-                (mv res memo)))))
-  (define svexlist-eval-memo ((x svexlist-p)
-                              (env svex-env-p)
-                              (memo svex-memotable-p))
-    :returns (mv (res 4veclist-p)
-                 (memo1 svex-memotable-p))
-    :measure (svexlist-count x)
-    (b* ((memo (svex-memotable-fix memo))
-         ((when (atom x)) (mv nil memo))
-         ((mv first memo) (svex-eval-memo (car x) env memo))
-         ((mv rest memo) (svexlist-eval-memo (cdr x) env memo)))
-      (mv (cons first rest) memo)))
-  ///
-  (deffixequiv-mutual svex-eval-memo)
-  (verify-guards svex-eval-memo)
-
-  (defun-sk svex-eval-memotable-ok (memo env)
-    (forall x
-            (implies (hons-assoc-equal x (svex-memotable-fix memo))
-                     (equal (cdr (hons-assoc-equal x (svex-memotable-fix memo)))
-                            (svex-eval x env))))
-    :rewrite :direct)
-
-  (in-theory (disable svex-eval-memotable-ok
-                      svex-eval-memotable-ok-necc))
-  (local (in-theory (enable svex-eval-memotable-ok-necc)))
-
-  (defthm svex-eval-memotable-ok-empty
-    (svex-eval-memotable-ok nil env)
-    :hints(("Goal" :in-theory (enable svex-eval-memotable-ok))))
-
-  (defthm svex-eval-memotable-ok-fix
-    (implies (svex-eval-memotable-ok memo env)
-             (svex-eval-memotable-ok (svex-memotable-fix memo) env))
-    :hints(("Goal" :expand ((svex-eval-memotable-ok (svex-memotable-fix memo) env)))))
-
-  (defthm svex-eval-memotable-ok-extend
-    (implies (and (svex-eval-memotable-ok memo env)
-                  (equal val (svex-eval x env)))
-             (svex-eval-memotable-ok
-              (cons (cons x val) memo) env))
-    :hints (("goal" :expand ((svex-eval-memotable-ok
-                              (cons (cons x (svex-eval x env)) memo) env)))))
-
-  (local (in-theory (disable svex-eval-memo svexlist-eval-memo)))
-
-  (defthm-svex-eval-memo-flag
-    (defthm svex-eval-memo-correct
-      (b* (((mv res memo1) (svex-eval-memo x env memo)))
-        (implies (svex-eval-memotable-ok memo env)
-                 (and (svex-eval-memotable-ok memo1 env)
-                      (equal res (svex-eval x env)))))
-      :hints ('(:expand ((svex-eval-memo x env memo)
-                         (svex-eval x env))))
-      :flag svex-eval-memo)
-    (defthm svexlist-eval-memo-correct
-      (b* (((mv res memo1) (svexlist-eval-memo x env memo)))
-        (implies (svex-eval-memotable-ok memo env)
-                 (and (svex-eval-memotable-ok memo1 env)
-                      (equal res (svexlist-eval x env)))))
-      :hints ('(:expand ((svexlist-eval-memo x env memo)
-                         (svexlist-eval x env))))
-      :flag svexlist-eval-memo)))
 
 
 
-(defalist svar-boolmasks :key-type svar :val-type integerp)
+(defalist svar-boolmasks
+  :key-type svar
+  :val-type integerp)
 
 (define svar-boolmasks-lookup ((v svar-p) (boolmasks svar-boolmasks-p))
   :returns (boolmask integerp :rule-classes :type-prescription)
@@ -579,45 +545,32 @@ has one possible value.</p>"
 
 
 
-(make-event
- `(encapsulate nil
-    (set-ignore-ok t)
-    (defthm svex-eval-of-quoted
-      (implies (syntaxp (quotep x))
-               (equal (svex-eval x env)
-                      ,(acl2::body 'svex-eval nil (w state))))
-      :hints(("Goal" :in-theory (enable svex-eval))))))
-
-(defthm svex-eval-of-svex-call
-  (equal (svex-eval (svex-call fn args) env)
-         (svex-apply fn (svexlist-eval args env)))
-  :hints(("Goal" :expand ((svex-eval (svex-call fn args) env)))))
-
-(defthm svex-eval-when-fncall
-  (implies (equal (svex-kind x) :call)
-           (equal (svex-eval x env)
-                  (svex-apply (svex-call->fn x)
-                              (svexlist-eval (svex-call->args x) env))))
-  :hints(("Goal" :in-theory (enable svex-eval))))
-
-(defthm svex-eval-when-quote
-  (implies (eq (svex-kind x) :quote)
-           (equal (svex-eval x env)
-                  (svex-quote->val x)))
-  :hints(("Goal" :in-theory (enable svex-eval))))
 
 
-(defthm svexlist-eval-of-cons
-  (equal (svexlist-eval (cons a b) env)
-         (cons (svex-eval a env)
-               (svexlist-eval b env)))
-  :hints(("Goal" :in-theory (enable svexlist-eval))))
 
 
-(defthm 4veclist-nth-of-cons
-  (implies (syntaxp (quotep n))
-           (equal (4veclist-nth n (cons a b))
-                  (if (zp n)
-                      (4vec-fix a)
-                    (4veclist-nth (1- n) b))))
-  :hints(("Goal" :in-theory (enable 4veclist-nth))))
+
+
+(defsection svcall
+  :parents (svex)
+  :short "Safely construct an @(see svex) for a function call."
+
+  :long "<p>@('(call svcall)') just constructs an @(see svex) that applies
+@('fn') to the given @('args').  This macro is ``safe'' in that, at compile
+time, it ensures that @('fn') is one of the known functions (see the @(see
+svex-functions)) and that it is being given the right number of arguments.</p>
+
+@(def svcall)"
+
+  (defun svcall-fn (fn args)
+    (declare (xargs :guard t))
+    (b* ((look (assoc fn *svex-op-table*))
+         ((unless look)
+          (er hard? 'svcall "Svex function doesn't exist: ~x0" fn))
+         (formals (third look))
+         ((unless (eql (len formals) (len args)))
+          (er hard? 'svcall "Wrong arity for call of ~x0" fn)))
+      `(svex-call ',fn (list . ,args))))
+
+  (defmacro svcall (fn &rest args)
+    (svcall-fn fn args)))
