books/centaur/sv/svex/junk.lisp
@@ -1,0 +1,127 @@
+; SV - Symbolic Vector Hardware Analysis Framework
+; Copyright (C) 2014-2015 Centaur Technology
+;
+; Contact:
+;   Centaur Technology Formal Verification Group
+;   7600-C N. Capital of Texas Highway, Suite 300, Austin, TX 78731, USA.
+;   http://www.centtech.com/
+;
+; License: (An MIT/X11-style license)
+;
+;   Permission is hereby granted, free of charge, to any person obtaining a
+;   copy of this software and associated documentation files (the "Software"),
+;   to deal in the Software without restriction, including without limitation
+;   the rights to use, copy, modify, merge, publish, distribute, sublicense,
+;   and/or sell copies of the Software, and to permit persons to whom the
+;   Software is furnished to do so, subject to the following conditions:
+;
+;   The above copyright notice and this permission notice shall be included in
+;   all copies or substantial portions of the Software.
+;
+;   THE SOFTWARE IS PROVIDED "AS IS", WITHOUT WARRANTY OF ANY KIND, EXPRESS OR
+;   IMPLIED, INCLUDING BUT NOT LIMITED TO THE WARRANTIES OF MERCHANTABILITY,
+;   FITNESS FOR A PARTICULAR PURPOSE AND NONINFRINGEMENT. IN NO EVENT SHALL THE
+;   AUTHORS OR COPYRIGHT HOLDERS BE LIABLE FOR ANY CLAIM, DAMAGES OR OTHER
+;   LIABILITY, WHETHER IN AN ACTION OF CONTRACT, TORT OR OTHERWISE, ARISING
+;   FROM, OUT OF OR IN CONNECTION WITH THE SOFTWARE OR THE USE OR OTHER
+;   DEALINGS IN THE SOFTWARE.
+;
+; Original author: Sol Swords <sswords@centtech.com>
+
+(in-package "SV")
+(include-book "evaluator")
+
+
+;; junk.lisp -- bozo are we using any of this?
+
+
+(defalist svex-memotable :key-type svex :val-type 4vec)
+
+(defthm 4vec-p-lookup-in-svex-memotable
+  (implies (and (svex-memotable-p x)
+                (hons-assoc-equal k x))
+           (4vec-p (cdr (hons-assoc-equal k x)))))
+
+(defines svex-eval-memo
+  ;; Self-memoized version of svex-eval, for GL
+  :verify-guards nil
+  (define svex-eval-memo ((x svex-p)
+                          (env svex-env-p)
+                          (memo svex-memotable-p))
+    :returns (mv (res 4vec-p)
+                 (memo1 svex-memotable-p))
+    :measure (svex-count x)
+    (b* ((memo (svex-memotable-fix memo)))
+      (svex-case x
+        :quote (mv x.val memo)
+        :var (mv (svex-env-fastlookup x.name env) memo)
+        :call (b* ((x (svex-fix x))
+                   (look (hons-get x memo))
+                   ((when look) (mv (cdr look) memo))
+                   ((mv args memo) (svexlist-eval-memo x.args env memo))
+                   (res (svex-apply x.fn args))
+                   (memo (hons-acons x res memo)))
+                (mv res memo)))))
+  (define svexlist-eval-memo ((x svexlist-p)
+                              (env svex-env-p)
+                              (memo svex-memotable-p))
+    :returns (mv (res 4veclist-p)
+                 (memo1 svex-memotable-p))
+    :measure (svexlist-count x)
+    (b* ((memo (svex-memotable-fix memo))
+         ((when (atom x)) (mv nil memo))
+         ((mv first memo) (svex-eval-memo (car x) env memo))
+         ((mv rest memo) (svexlist-eval-memo (cdr x) env memo)))
+      (mv (cons first rest) memo)))
+  ///
+  (deffixequiv-mutual svex-eval-memo)
+  (verify-guards svex-eval-memo)
+
+  (defun-sk svex-eval-memotable-ok (memo env)
+    (forall x
+            (implies (hons-assoc-equal x (svex-memotable-fix memo))
+                     (equal (cdr (hons-assoc-equal x (svex-memotable-fix memo)))
+                            (svex-eval x env))))
+    :rewrite :direct)
+
+  (in-theory (disable svex-eval-memotable-ok
+                      svex-eval-memotable-ok-necc))
+  (local (in-theory (enable svex-eval-memotable-ok-necc)))
+
+  (defthm svex-eval-memotable-ok-empty
+    (svex-eval-memotable-ok nil env)
+    :hints(("Goal" :in-theory (enable svex-eval-memotable-ok))))
+
+  (defthm svex-eval-memotable-ok-fix
+    (implies (svex-eval-memotable-ok memo env)
+             (svex-eval-memotable-ok (svex-memotable-fix memo) env))
+    :hints(("Goal" :expand ((svex-eval-memotable-ok (svex-memotable-fix memo) env)))))
+
+  (defthm svex-eval-memotable-ok-extend
+    (implies (and (svex-eval-memotable-ok memo env)
+                  (equal val (svex-eval x env)))
+             (svex-eval-memotable-ok
+              (cons (cons x val) memo) env))
+    :hints (("goal" :expand ((svex-eval-memotable-ok
+                              (cons (cons x (svex-eval x env)) memo) env)))))
+
+  (local (in-theory (disable svex-eval-memo svexlist-eval-memo)))
+
+  (defthm-svex-eval-memo-flag
+    (defthm svex-eval-memo-correct
+      (b* (((mv res memo1) (svex-eval-memo x env memo)))
+        (implies (svex-eval-memotable-ok memo env)
+                 (and (svex-eval-memotable-ok memo1 env)
+                      (equal res (svex-eval x env)))))
+      :hints ('(:expand ((svex-eval-memo x env memo)
+                         (svex-eval x env))))
+      :flag svex-eval-memo)
+    (defthm svexlist-eval-memo-correct
+      (b* (((mv res memo1) (svexlist-eval-memo x env memo)))
+        (implies (svex-eval-memotable-ok memo env)
+                 (and (svex-eval-memotable-ok memo1 env)
+                      (equal res (svexlist-eval x env)))))
+      :hints ('(:expand ((svexlist-eval-memo x env memo)
+                         (svexlist-eval x env))))
+      :flag svexlist-eval-memo)))
+
