books/centaur/sv/svex/top.lisp
@@ -46,4 +46,4 @@
 (include-book "svmask")
 (include-book "symbolic")
 (include-book "vars")
-
+(include-book "xeval")
