books/centaur/sv/svex/xeval.lisp
@@ -1,0 +1,179 @@
+; SV - Symbolic Vector Hardware Analysis Framework
+; Copyright (C) 2014-2015 Centaur Technology
+;
+; Contact:
+;   Centaur Technology Formal Verification Group
+;   7600-C N. Capital of Texas Highway, Suite 300, Austin, TX 78731, USA.
+;   http://www.centtech.com/
+;
+; License: (An MIT/X11-style license)
+;
+;   Permission is hereby granted, free of charge, to any person obtaining a
+;   copy of this software and associated documentation files (the "Software"),
+;   to deal in the Software without restriction, including without limitation
+;   the rights to use, copy, modify, merge, publish, distribute, sublicense,
+;   and/or sell copies of the Software, and to permit persons to whom the
+;   Software is furnished to do so, subject to the following conditions:
+;
+;   The above copyright notice and this permission notice shall be included in
+;   all copies or substantial portions of the Software.
+;
+;   THE SOFTWARE IS PROVIDED "AS IS", WITHOUT WARRANTY OF ANY KIND, EXPRESS OR
+;   IMPLIED, INCLUDING BUT NOT LIMITED TO THE WARRANTIES OF MERCHANTABILITY,
+;   FITNESS FOR A PARTICULAR PURPOSE AND NONINFRINGEMENT. IN NO EVENT SHALL THE
+;   AUTHORS OR COPYRIGHT HOLDERS BE LIABLE FOR ANY CLAIM, DAMAGES OR OTHER
+;   LIABILITY, WHETHER IN AN ACTION OF CONTRACT, TORT OR OTHERWISE, ARISING
+;   FROM, OUT OF OR IN CONNECTION WITH THE SOFTWARE OR THE USE OR OTHER
+;   DEALINGS IN THE SOFTWARE.
+;
+; Original author: Sol Swords <sswords@centtech.com>
+
+(in-package "SV")
+(include-book "evaluator")
+
+
+(defines svex-xeval
+  :parents (evaluation)
+  :short "Cheaply detect always-constant bits in an @(see svex) by
+approximately evaluating it under the empty (i.e., all X) environment."
+
+  :long "<p>This is a lightweight way to tell that certain bits of an @(see
+svex) expression are actually particular constants, no matter how you bind its
+variables.  It returns an @(see 4vec) which tells us that certain bits of
+@('expr') are ``obviously'' constant, and that other bits are not known to be
+constant.  In particular:</p>
+
+<ul>
+
+<li>Xes indicate that this bit of @('expr') is not obviously constant,</li>
+
+<li>0/1/Z bits indicate that this bit of @('expr') is obviously always
+0/1/Z.</li>
+
+</ul>
+
+
+<h3>Example</h3>
+
+<p>Consider the following expression:</p>
+
+@({
+     (bitand (bitor a b) (bitand c #b1000))
+})
+
+<p>What values can this expression return?  You can see that, regardless of the
+values of @('a'), @('b'), and @('c'), the resulting @(see 4vec) will always
+have 0 on its lower 3 bits.  It will also always have 0s on bits 5 and above.
+But bit 4 will depend on the values of @('a'), @('b'), and @('c').</p>
+
+<p>When we use @('svex-xeval'), we get:</p>
+
+@({
+     (svex-xeval '(bitand (bitor a b) (bitand c #b1000))) == (8 . 0)
+})
+
+<p>Here is the interpretation of the resulting @(see 4vec), @('(8 . 0)'):</p>
+
+@({
+     bits of upper (8) are: 0...01000
+     bits of lower (0) are: 0...00000
+     ---------------------------------
+     01ZX interpretation:   0...0X000
+})
+
+<p>So @('svex-xeval') is telling us that:</p>
+
+<ul>
+<li>Bit 4 is not known to be always constant.</li>
+<li>All the other bits are known to be always constant 0.</li>
+</ul>
+
+
+<h3>Implementation</h3>
+
+<p>@('(svex-xeval expr)') is almost identical to @('(svex-eval expr nil)').
+Recall that, when @(see svex-eval) encounters a variable that isn't bound in
+the environment, it returns the all Xes vector.  So, when we evaluate @('expr')
+in the @('nil') environment, it's as if we've bound all of its variables to all
+Xes.</p>
+
+<p>If all of our @(see expressions) were ``properly monotonic'' and truly
+treated @('x') bits as unknowns, then the result of @('(svex-eval expr nil)')
+would clearly be a conservative approximation of @('(svex-eval expr env)') for
+any environment.</p>
+
+<p>This almost works.  However, the case-equality operator @('===') is
+problematic, because it has a non-monotonic semantics that does not treat X
+bits as unknown.  As a result, evaluation in the @('nil') environment doesn't
+really work for what we're trying to do here.  For example:</p>
+
+@({
+     (svex-eval '(=== a b) nil)     -->  -1  (all bits true)
+})
+
+<p>But obviously this expression isn't always true, for instance:</p>
+
+@({
+    (let ((env '((a . 1) (b . 0))))
+      (svex-eval '(=== a b) env))    -->  0  (all bits false)
+})
+
+<p>To correct for this, @('svex-xeval') simply interprets @('===') as @('==')
+instead.  Since @('==') is an ordinary, properly monotonic function, and
+since it conservatively approximates @('==='), this works out quite well
+and we get, for instance:</p>
+
+@({
+     (svex-xeval '(=== a b))  --> all Xes
+     (svex-xeval '(=== a a))  --> all Xes
+     (svex-xeval '(=== 0 0))  --> all true
+})"
+
+  (define svex-xeval ((expr svex-p "Expression to evaluate."))
+    :returns (val 4vec-p "Indication of always-constant bits (see below).")
+    :measure (svex-count expr)
+    :verify-guards nil
+    (svex-case expr
+      :quote expr.val
+      :var (4vec-x)
+      :call (svex-apply
+             (if (eq expr.fn '===)
+                 '==
+               expr.fn)
+             (svexlist-xeval expr.args))))
+
+  (define svexlist-xeval ((x svexlist-p))
+    :measure (svexlist-count x)
+    :returns (val 4veclist-p)
+    :short "Maps @(see svex-xeval) over an @(see svex) list."
+    (if (atom x)
+        nil
+      (cons (svex-xeval (car x))
+            (svexlist-xeval (cdr x)))))
+  ///
+  (verify-guards svex-xeval)
+  (memoize 'svex-xeval :condition '(eq (svex-kind expr) :call))
+
+  (deffixequiv-mutual svex-xeval
+    :hints (("goal" :expand ((svexlist-fix x)))))
+
+  (defthm svexlist-xeval-nil
+    (equal (svexlist-xeval nil) nil))
+
+  (defthm car-of-svexlist-xeval
+    (4vec-equiv (car (svexlist-xeval x))
+                (svex-xeval (car x))))
+
+  (defthm cdr-of-svexlist-xeval
+    (4veclist-equiv (cdr (svexlist-xeval x))
+                    (svexlist-xeval (cdr x))))
+
+  (defthm len-of-svexlist-xeval
+    (equal (len (svexlist-xeval x))
+           (len x)))
+
+  (defthm svexlist-xeval-of-append
+    (equal (svexlist-xeval (append a b))
+           (append (svexlist-xeval a)
+                   (svexlist-xeval b)))
+    :hints(("Goal" :in-theory (enable append)))))
